TM/Compound/MoveToSymbol.v
@@ -1,0 +1,211 @@
+Require Import TM.Prelim.
+Require Import TM.Basic.Mono.
+Require Import TM.Combinators.Match TM.Combinators.While TM.Combinators.SequentialComposition.
+
+Section move_to_symbol.
+  
+  Variable sig : finType.
+  Variable f : sig -> bool.
+
+  Print Mono.
+
+  Definition M1 D : { M : mTM sig 1 & states M -> bool * bool } :=
+    MATCH (TEST_CHAR f)
+          (fun b => match b with
+                 | Some false => Move sig D ;; mono_Nop sig (true, false) (* Not found yet: move on and continue *)
+                 | Some true => mono_Nop sig (false, true) (* Found: stop *)
+                 | None => mono_Nop sig (false, false) (* Reached end of tape: stop *)
+                 end).
+
+
+  (* Returns true if symbol was found, false otherwise *)
+  Definition move_to_symbol D : { M : mTM sig 1 & states M -> bool } := WHILE (M1 D).
+
+  Fixpoint to_symbol_list_r l1 l2 :=
+    match (l2,l1) with
+    | ([],[]) => (false, niltape _)
+    | ([], c :: l) => (false, rightof c l)
+    | (c :: l, l1) => if f c then (true, midtape l1 c l) else to_symbol_list_r (c :: l1) l
+    end.
+
+  (* Careful: if the cursor is left of the tape, nothing will happen! *)
+  Fixpoint to_symbol_r t :=
+    match t with
+    | niltape _ => (false, niltape _)
+    | leftof c r => (false, leftof c r)
+    | rightof c r => (false, rightof c r)
+    | midtape l1 c l2 => to_symbol_list_r l1 (c :: l2)
+    end.
+
+  Definition R_move_to_symbol_r : Rel (tapes sig 1) (FinType (EqType bool) * tapes sig 1) :=
+    Mk_R_p (fun t t' => t' = to_symbol_r t).
+
+
+  Lemma to_symbol_r_current_Some t s :
+    f s = true -> current t = Some s -> to_symbol_r t = (true, t).
+  Proof.
+    intros. destruct t; cbn in *; try congruence. inv H0. now rewrite H.
+  Qed.
+
+  Lemma to_symbol_r_current_None t :
+    current t = None -> to_symbol_r t = (false, t).
+  Proof.
+    intros. destruct t; cbn in *; try congruence.
+  Qed.
+
+  Lemma to_symbol_r_move_false t t' s :
+    current t = Some s -> f s = false -> t' = tape_move_mono t (None, R) -> to_symbol_r t = to_symbol_r t'.
+  Proof.
+    intros H1 H2 ->. destruct t; cbn in *; try congruence. inv H1. rewrite H2. cbn. destruct l0; cbn; auto.
+  Qed.
+  
+  (* TODO: This proof should be monstly automatised *)
+  Lemma move_to_symbol_r_WRealise :
+    move_to_symbol R ⊫ R_move_to_symbol_r.
+  Proof.
+    eapply WRealise_monotone.
+    - eapply While_WRealise. unfold M1. eapply Match_WRealise.
+      eapply Realise_WRealise. eapply RealiseIn_Realise. eapply test_chr_Sem.
+      instantiate (1 := fun o => match o with Some true => _ | Some false => _ | None => _ end).
+      intros [ [ | ] | ].
+      + eapply Realise_WRealise, RealiseIn_Realise. eapply mono_Nop_Sem.
+      + eapply Realise_WRealise. eapply Seq_Realise; eapply RealiseIn_Realise. eapply Move_Sem. eapply mono_Nop_Sem.
+      + eapply Realise_WRealise, RealiseIn_Realise. eapply mono_Nop_Sem.
+    - intros tin (bout, tout). cbn in bout. intros H. hnf in *. destruct H as (t1&H1&f'&t2&(H2&H3)&H4). hnf in *.
+      induction H1 as [x | x y z IH1 IH2 IH3].
+      + destruct f'.
+        * destruct H3 as (s&H3&H3'). subst. destruct (f s) eqn:E; hnf in *.
+          -- destruct H4 as (H4&H4'). hnf in *. subst. inv H4. cbn. erewrite to_symbol_r_current_Some; eauto. now rewrite H2.
+          -- destruct H4 as ((b2&t3)&H4&H4'). hnf in *. destruct b2 eqn:E2; hnf in *.
+             ++ destruct H4 as (H41&c&H42). destruct H4' as (H4&->); hnf in *. congruence.
+             ++ destruct H4 as (H41&H42); hnf in *. destruct H4' as (H4&->); hnf in *. congruence.
+        * hnf in *. destruct H4 as (H4&->); hnf in *. inv H4. rewrite <- H2. now erewrite to_symbol_r_current_None; eauto.
+      + hnf in *. rewrite H2 in *. clear H2.
+        destruct IH1 as (b1&ob&t&(H1&H1')&H1''). hnf in *. rewrite H1 in *; clear H1. destruct ob as [ [ ] | ]; hnf in *.
+        * destruct H1' as (s&H1&H1'). hnf in *. destruct H1'' as (H1''&->). hnf in *. congruence.
+        * destruct H1' as (s&H1&H2). destruct H1'' as ((q&t3)&H5&H6). hnf in *. destruct H6 as (H6&H7). hnf in *. subst. inv H6. 
+          specialize (IH3 eq_refl). destruct q; hnf in *.
+          -- destruct H5 as (H5&s'&H6). hnf in *.
+             destruct f'.
+             ++ destruct H3 as (s''&H3&H3'); subst. rewrite IH3; [clear IH3 | eauto]. destruct (f s''); hnf in *.
+                ** destruct H4 as (H4&->). hnf in *. inv H4. rewrite H1 in H6. inv H6. erewrite (to_symbol_r_move_false H1); eauto.
+                ** destruct H4 as ((f2, t3)&H4&H7). hnf in *. destruct H7 as (H7&H8). hnf in *. congruence.
+             ++ specialize (IH3 H3). rewrite IH3. hnf in *. destruct H4 as (H4&->). hnf in *. inv H4.
+                rewrite H5. symmetry. eapply (to_symbol_r_move_false H1); eauto.
+          -- destruct H5 as (H5&->). congruence.
+        * destruct H1'' as (H1''&->). hnf in *. congruence.
+  Qed.
+
+  Fixpoint time_symbol_list l1 l2 :=
+    match (l2,l1) with
+    | ([],[]) => 1
+    | ([], c :: l) => 1
+    | (c :: l, l1) => 1 + if f c then 0 else 1 + time_symbol_list (c :: l1) l
+    end.
+
+  Fixpoint time_until_symbol t :=
+    match t with
+    | niltape _ => 1
+    | leftof c r => 1
+    | rightof c r => 1
+    | midtape l1 c l2 => time_symbol_list l1 (c :: l2)
+    end.
+
+  (*
+  Lemma m1_term_cannonical : { T : tapes sig 1 -> nat -> Type & projT1 (M1 R) ⇓ T }.
+  Proof.
+    eexists. cbn. eapply Match_Terminates.
+    instantiate (1 := fun o => match o with Some true => _ | Some false => _ | None => _ end). cbn.
+    intros [ [ | ] | ]; cbn.
+    - eapply 
+
+  Lemma move_to_sym_r_term_cannonical : { T : tapes sig 1 -> nat -> Type & projT1 (move_to_symbol R) ⇓ T }.
+  Proof.
+    eexists. cbn. eapply While_Terminates. Unshelve. shelve.
+    cbn. eapply Match_Terminates.
+
+  Lemma move_to_symbol_r_term :
+    projT1 (move_to_symbol R) ⇓ (fun x i => i >= 3 * time_until_symbol (x[@Fin.F1])).
+  Proof.
+    eapply TerminatesIn_monotone.
+    - cbn -[M1]. eapply While_Terminates.
+      Unshelve. shelve. cbn.
+      pose proof (Match_Terminates (*T__f := fun o => match o with Some true => _ | Some false => _ | None => _ end*)) as L.
+      specialize (L 1 sig (FinType (EqType (bool)))).
+
+    
+    TMcorrect.
+    - unfold MoveR.
+      eapply functionalOn_lift.
+      hnf.
+      intros ? ? ? ([] & ? ) ([] & ?) ? ?; firstorder congruence.
+    - intros. intuition. unfold liftT in H.
+      destruct (get_at is_a_tape x) eqn:E.
+      + cbn in *. exists x, false, i. firstorder. left. rewrite E. firstorder. 
+      + cbn in *. exists x, false, i. firstorder. left. rewrite E. firstorder. 
+      + cbn in *. exists x, false, i. firstorder. left. rewrite E. firstorder. 
+      + cbn in *. destruct (f e) eqn:E2.
+        * exists x, false, i. firstorder. right. rewrite E. firstorder. 
+        * exists (tape_move_multi x (do_on_tape is_a_tape (None, TM.R))). exists true. exists 3.
+          { split. split.
+            * simpl_TM. now rewrite E. 
+            * intuition. simpl_TM.
+            * simpl_TM.
+              unfold liftT.
+              rewrite !get_at_tape_move_multi.
+              simpl_TM.
+              rewrite !E. simpl_TM. cbn. instantiate (1 := 0). cbn.
+              destruct l0; cbn in *; omega. 
+          }
+  Qed.
+  *)
+
+  
+
+  (* TODO: Move to left *)
+  (* Idee: Tape-Reversierung *)
+  
+  Fixpoint to_symbol_list_l l1 l2 {struct l2} :=
+    match (l2,l1) with
+    | ([],[]) => (false, niltape _)
+    | ([], c :: l) => (false, leftof c l)
+    | (c :: l, l1) => if f c then (true, midtape l c l1) else to_symbol_list_l (c :: l1) l
+    end.
+
+  (* Careful: if the cursor is left of the tape, nothing will happen! *)
+  Fixpoint to_symbol_l t :=
+    match t with
+    | niltape _ => (false, niltape _)
+    | leftof c r => (false, leftof c r)
+    | rightof c r => (false, rightof c r)
+    | midtape l1 c l2 => to_symbol_list_l l2 (c :: l1)
+    end.
+
+  Lemma to_symbol_list_l_in_iff l1 l2 :
+    (exists s, s el l2 /\ f s = true) <-> (exists t', to_symbol_list_l l1 l2 = (true, t')).
+  Proof.
+    split; revert l1; induction l2; intros; cbn in *.
+    - destruct H as (s&H&H'). auto.
+    - destruct H as (s&[->|H]&H').
+      + rewrite H'. eauto.
+      + destruct (IHl2 (a :: l1)) as (t'&Ht'); eauto. destruct (f a); eauto.
+    - destruct H as (t'&H). destruct l1; congruence.
+    - destruct H as (t'&H). destruct (f a) eqn:E.
+      + inv H. eauto.
+      + destruct (IHl2 (a :: l1)) as (s&IH&IH'); eauto.
+  Qed.
+
+  Lemma to_symbol_l_false t t' :
+    to_symbol_l t = (false, t') ->
+    forall s, current t = Some s \/ ((exists s', current t = Some s') /\ s el left t) -> f s = false.
+  Proof.
+    revert t'. intros H. destruct t eqn:E; cbn in *; intros; firstorder; (intuition; try congruence).
+    - inv H1. destruct f eqn:E; auto. congruence.
+    - inv H1. 
+  Abort.
+
+  Definition R_move_to_symbol_l : Rel (tapes sig 1) (FinType (EqType bool) * tapes sig 1) :=
+    Mk_R_p (fun t t' => t' = to_symbol_l t).
+
+
+End move_to_symbol.
